Tactic_Inline.thy
@@ -19,9 +19,117 @@ using assms unfolding obs_eq'_def obs_eq_def rhoare_def denotation_callproc_rena
 thm obs_eq'_rename_variables_proc[of _ _ "[]"]
  *)
 
-lemma local_variable_name_renaming1: "local_variable_name_renaming [] ` x == x" 
-  unfolding local_variable_name_renaming_def[THEN ext] apply auto
-  by (smt UnCI inf_sup_distrib1 le_iff_inf mem_Collect_eq subsetI)
+locale callproc_conditions_simp begin
+
+definition "filter_global' == filter vu_global"
+definition "filter_local' == filter (\<lambda>x. \<not> vu_global x)"
+
+
+lemma local_variable_name_renaming_nil: "local_variable_name_renaming [] ` x == x" 
+  unfolding local_variable_name_renaming_def[THEN ext] by auto
+
+(* lemma local_variable_name_renaming2: "local_variable_name_renaming (a#b) ` X == local_variable_name_renaming b ` local_variable_name_renaming1 a ` X" 
+  unfolding local_variable_name_renaming_def
+  by (simp add: o_def image_image) *)
+
+lemma local_variable_name_renaming_union: "local_variable_name_renaming (a#b) ` (A \<union> B) == local_variable_name_renaming (a#b) ` A \<union> local_variable_name_renaming (a#b) ` B"
+  by (simp add: image_Un)
+
+lemma local_variable_name_renaming_insert: "local_variable_name_renaming (a#b) ` (insert x X) == insert (local_variable_name_renaming (a#b) x) (local_variable_name_renaming (a#b) ` X)"
+  by simp
+
+lemma local_variable_name_renaming_set: "local_variable_name_renaming (a#b) ` (set X) == set (map (local_variable_name_renaming (a#b)) X)"
+  by simp
+
+lemma local_variable_name_renaming_cons: "map (local_variable_name_renaming (a#b)) (x#X) == local_variable_name_renaming (a#b) x # map (local_variable_name_renaming (a#b)) X"
+  by simp
+
+lemma local_variable_name_renaming_nil2: "map (local_variable_name_renaming R) [] == []"
+  by simp
+
+
+lemma callproc_goal4: "local_variable_name_renaming ren ` filter_global X \<subseteq> Y \<union> Collect vu_global"
+  unfolding filter_global_def by auto
+
+(*lemma callproc_conditions_simp1b: "local_variable_name_renaming ren ` filter_global X \<subseteq> Y \<union> Collect vu_global == True"
+  apply (rule eq_reflection) unfolding filter_global_def by auto
+
+lemma callproc_conditions_simp1c: "local_variable_name_renaming1 ren ` filter_global X \<subseteq> Y \<union> Collect vu_global == True"
+  apply (rule eq_reflection)
+  by (auto simp: filter_global_def local_variable_name_renaming1_fix_globals)*)
+
+lemma filter_global': "filter_global (set X) == set (filter_global' X)"
+  unfolding filter_global_def filter_global'_def by simp
+
+lemma filter_local': "filter_local (set X) == set (filter_local' X)"
+  unfolding filter_local_def filter_local'_def by simp
+
+lemma filter_global'_nil: "filter_global' [] == []"
+  unfolding filter_global'_def by simp
+
+lemma filter_global'_cons1: "filter_global' (mk_variable_untyped (Variable n :: 'a::prog_type variable) # X) ==
+                             mk_variable_untyped (Variable n :: 'a variable) # filter_global' X"
+  unfolding filter_global'_def by auto 
+
+lemma filter_global'_cons2: "filter_global' (mk_variable_untyped (LVariable n :: 'a::prog_type variable) # X) ==
+                             filter_global' X"
+  unfolding filter_global'_def by auto 
+
+lemma filter_local'_nil: "filter_local' [] == []"
+  unfolding filter_local'_def by simp
+
+lemma filter_local'_cons1: "filter_local' (mk_variable_untyped (LVariable n :: 'a::prog_type variable) # X) ==
+                             mk_variable_untyped (LVariable n :: 'a variable) # filter_local' X"
+  unfolding filter_local'_def by auto 
+
+lemma filter_local'_cons2: "filter_local' (mk_variable_untyped (Variable n :: 'a::prog_type variable) # X) ==
+                             filter_local' X"
+  unfolding filter_local'_def by auto 
+
+lemma filter_local_union: "filter_local (X \<union> Y) == filter_local X \<union> filter_local Y"
+  apply (rule eq_reflection) unfolding filter_local_def by auto
+
+lemma filter_local_insert1: "filter_local (insert (mk_variable_untyped (LVariable n :: 'a::prog_type variable)) X) == 
+      insert (mk_variable_untyped (LVariable n :: 'a::prog_type variable)) (filter_local X)"
+  apply (rule eq_reflection) unfolding filter_local_def by auto
+  
+lemma filter_local_empty: "filter_local {} == {}"
+  apply (rule eq_reflection) unfolding filter_local_def by auto
+
+lemma local_variable_name_renaming_same: 
+  "local_variable_name_renaming ((a,b)#X) (mk_variable_untyped (LVariable a :: 'a::prog_type variable))
+      == mk_variable_untyped (LVariable b :: 'a variable)"
+  by later
+
+(* TODO how to make the simplifier use this? *)
+lemma local_variable_name_renaming_notsame: 
+  assumes "a\<noteq>x" and "b\<noteq>x"
+  shows "local_variable_name_renaming ((a,b)#X) (mk_variable_untyped (LVariable x :: 'a::prog_type variable))
+      == mk_variable_untyped (LVariable x :: 'a variable)"
+  by later
+
+lemmas callproc_conditions_simp =  
+  filter_global' filter_global'_cons1 filter_global'_cons2
+  filter_global'_nil filter_local_union filter_local' vars_variable_pattern[THEN eq_reflection]
+  filter_local'_cons1 filter_local'_cons2 filter_local'_nil filter_local_insert1
+  filter_local_empty local_variable_name_renaming_insert local_variable_name_renaming_union
+  local_variable_name_renaming_nil local_variable_name_renaming_same image_empty[THEN eq_reflection]
+  vars_unit_pattern[THEN eq_reflection] vars_pair_pattern[THEN eq_reflection] 
+  append_Cons[THEN eq_reflection] append_Nil[THEN eq_reflection]
+  rename_local_variables_pattern_id[THEN eq_reflection]
+  local_variable_name_renaming_set local_variable_name_renaming_cons 
+  local_variable_name_renaming_nil2 local_variable_name_renaming_notsame
+
+(* TODO remove *)
+lemma 
+  "local_variable_name_renaming [(''a'',''b'')] (mk_variable_untyped (LVariable ''x'' :: int variable))
+  = mk_variable_untyped (LVariable ''x'' :: int variable)"
+using[[simp_trace_new]]
+apply (simp add: callproc_conditions_simp)
+SORRY
+
+find_theorems "_ ` set _"
+end
 
 ML_file "tactic_inline.ML"
                                                                     
